Implement erase as inference rules

AST.v
@@ -40,29 +40,44 @@ Inductive ut_expr : Type := (* ut_expr : untyped expression *)
   | ut_Nil: ut_expr.
 
 Inductive t_expr : Type := (* t_expr : typed expression *)
-  | t_Num : nat -> t_expr
-  | t_Bool : bool -> t_expr
-  | t_Var : id -> t_expr
-  | t_If : t_expr -> t_expr -> t_expr -> t_expr
-  | t_Fun : id -> type -> t_expr -> t_expr
-  | t_Call : t_expr -> t_expr -> t_expr
-  | t_Binop : binop -> t_expr -> t_expr -> t_expr
-  | t_Cons : t_expr -> t_expr -> t_expr
-  | t_Nil : type -> t_expr.
+  | t_Num: nat -> t_expr
+  | t_Bool: bool -> t_expr
+  | t_Var: id -> t_expr
+  | t_If: t_expr -> t_expr -> t_expr -> t_expr
+  | t_Fun: id -> type -> t_expr -> t_expr
+  | t_Call: t_expr -> t_expr -> t_expr
+  | t_Binop: binop -> t_expr -> t_expr -> t_expr
+  | t_Cons: t_expr -> t_expr -> t_expr
+  | t_Nil: type -> t_expr.
 
 Definition environment := partial_map type.
 Definition constraint := list (type * type) % type.
 Definition substitution := list (id * type) % type.
 
-Fixpoint erase (t_ex : t_expr) : ut_expr :=
-  match t_ex with
-    | t_Num n => ut_Num n
-    | t_Bool b => ut_Bool b
-    | t_Var x => ut_Var x
-    | t_If c e1 e2 => ut_If (erase c) (erase e1) (erase e2)
-    | t_Fun x t e => ut_Fun x (erase e)
-    | t_Call f e => ut_Call (erase f) (erase e)
-    | t_Binop op e1 e2 => ut_Binop op (erase e1) (erase e2)
-    | t_Cons hd tl => ut_Cons (erase hd) (erase tl)
-    | t_Nil t => ut_Nil
-  end.
+Inductive erase : t_expr -> ut_expr -> Prop :=
+  | E_Num: forall n, erase (t_Num n) (ut_Num n)
+  | E_Bool: forall b, erase (t_Bool b) (ut_Bool b)
+  | E_Var: forall x, erase (t_Var x) (ut_Var x)
+  | E_If: forall c c_e e1 e1_e e2 e2_e,
+      erase c c_e ->
+      erase e1 e1_e ->
+      erase e2 e2_e ->
+      erase (t_If c e1 e2) (ut_If c_e e1_e e2_e)
+  | E_Fun: forall x t e e_e,
+      erase e e_e ->
+      erase (t_Fun x t e) (ut_Fun x e_e)
+  | E_Call: forall f f_e e e_e,
+      erase f f_e ->
+      erase e e_e ->
+      erase (t_Call f e) (ut_Call f_e e_e)
+  | E_Binop: forall op e1 e1_e e2 e2_e,
+      erase e1 e1_e ->
+      erase e2 e2_e ->
+      erase (t_Binop op e1 e2) (ut_Binop op e1_e e2_e)
+  | E_Cons: forall hd hd_e tl tl_e,
+      erase hd hd_e ->
+      erase tl tl_e ->
+      erase (t_Cons hd tl) (ut_Cons hd_e tl_e)
+  | E_Nil: forall t,
+      erase (t_Nil t) ut_Nil.
+
