Proofs.v
@@ -18,68 +18,80 @@ Require Import TypeChecker.
 (* Small proofs *)
 
 (* erase *)
-Example erase_num : forall n, erase (t_Num n) = ut_Num n.
-Proof. reflexivity. Qed.
+Lemma erase_num : forall n ut, erase (t_Num n) = ut <-> ut = ut_Num n.
+Proof.
+  intros. simpl.
+  split; try (intros; symmetry; assumption).
+Qed.
 
-Example erase_bool : forall b, erase (t_Bool b) = ut_Bool b.
-Proof. reflexivity. Qed.
+Lemma erase_bool : forall b ut, erase (t_Bool b)= ut <-> ut = ut_Bool b.
+Proof.
+  intros. simpl.
+  split; try (intros; symmetry; assumption).
+Qed.
 
-Example erase_var : forall x, erase (t_Var x) = ut_Var x.
-Proof. reflexivity. Qed.
+Lemma erase_var : forall x ut, erase (t_Var x) = ut <-> ut = ut_Var x.
+Proof.
+  intros. simpl.
+  split; try (intros; symmetry; assumption).
+Qed.
 
-Example erase_if : forall c_t c_ut e1_t e1_ut e2_t e2_ut,
+Lemma erase_if : forall c_t c_ut e1_t e1_ut e2_t e2_ut ut,
   erase c_t = c_ut ->
   erase e1_t = e1_ut ->
   erase e2_t = e2_ut ->
-  erase (t_If c_t e1_t e2_t) = ut_If c_ut e1_ut e2_ut.
+  (erase (t_If c_t e1_t e2_t) = ut <-> ut = ut_If c_ut e1_ut e2_ut).
 Proof.
   intros. simpl.
   rewrite H. rewrite H0. rewrite H1.
-  reflexivity.
+  split; try (intros; symmetry; assumption).
 Qed.
 
-Example erase_fun : forall x T e_t e_ut,
+Lemma erase_fun : forall x T e_t e_ut ut,
   erase e_t = e_ut ->
-  erase (t_Fun x T e_t) = ut_Fun x e_ut.
+  (erase (t_Fun x T e_t) = ut <-> ut = ut_Fun x e_ut).
 Proof.
   intros. simpl.
   rewrite H.
-  reflexivity.
+  split; try (intros; symmetry; assumption).
 Qed.
 
-Example erase_call : forall f_t f_ut e_t e_ut,
+Lemma erase_call : forall f_t f_ut e_t e_ut ut,
   erase f_t = f_ut ->
   erase e_t = e_ut ->
-  erase (t_Call f_t e_t) = ut_Call f_ut e_ut.
+  (erase (t_Call f_t e_t) = ut <-> ut = ut_Call f_ut e_ut).
 Proof.
   intros. simpl.
   rewrite H. rewrite H0.
-  reflexivity.
+  split; try (intros; symmetry; assumption).
 Qed.
 
-Example erase_binop : forall op e1_t e1_ut e2_t e2_ut,
+Lemma erase_binop : forall op e1_t e1_ut e2_t e2_ut ut,
   erase e1_t = e1_ut ->
   erase e2_t = e2_ut ->
-  erase (t_Binop op e1_t e2_t) = ut_Binop op e1_ut e2_ut.
+  (erase (t_Binop op e1_t e2_t) = ut <-> ut = ut_Binop op e1_ut e2_ut).
 Proof.
   intros. simpl.
   rewrite H. rewrite H0.
-  reflexivity.
+  split; try (intros; symmetry; assumption).
 Qed.
 
-Example erase_cons : forall hd_t hd_ut tl_t tl_ut,
+Lemma erase_cons : forall hd_t hd_ut tl_t tl_ut ut,
   erase hd_t = hd_ut ->
   erase tl_t = tl_ut ->
-  erase (t_Cons hd_t tl_t) = ut_Cons hd_ut tl_ut.
+  (erase (t_Cons hd_t tl_t) = ut <-> ut = ut_Cons hd_ut tl_ut).
 Proof.
   intros. simpl.
   rewrite H. rewrite H0.
-  reflexivity.
+  split; try (intros; symmetry; assumption).
 Qed.
 
-Example erase_nil : forall T,
-  erase (t_Nil T) = ut_Nil.
-Proof. reflexivity. Qed.
+Lemma erase_nil : forall T ut,
+  erase (t_Nil T) = ut <-> ut = ut_Nil.
+Proof.
+  intros. simpl.
+  split; try (intros; symmetry; assumption).
+Qed.
 
 (* app_substs *)
 Example app_substs_ex1 : app_substs [(Id 1, TNum)] (TFun (TVar (Id 1)) TNum) = TFun TNum TNum.
@@ -108,19 +120,36 @@ Qed.
 Theorem typeinference_soundness :
   forall (t : t_expr) (T : type)
     (e : ut_expr) (env : environment) (fv : nat) (S : type) (C : constraint),
-  env = (@empty type) ->
   erase t = e ->
   typecheck env t T ->
   typeinf env 0 e (fv, S, C) ->
-  (exists (s : substitution), solution s C /\ apply s S = T).
+  (exists (s : substitution), solution s C /\ app_substs s S = T).
 Proof.
+  intros t T e env fv S C He Htc Hti.
+  induction t.
+  - apply erase_num in He. rewrite He in Hti.
+    inversion Hti. inversion Htc.
+    exists []. simpl. split.
+    * apply S_Empty.
+    * reflexivity.
+  - apply erase_bool in He. rewrite He in Hti.
+    inversion Hti. inversion Htc.
+    exists []. simpl. split.
+    * apply S_Empty.
+    * reflexivity.
+  - admit.
+  - admit.
+  - admit.
+  - admit.
+  - admit.
+  - admit.
+  - admit.
 Admitted.
 
 Theorem typeinference_completeness :
   forall (e : ut_expr) (env : environment) (fv : nat) (S : type) (C :constraint) (s : substitution),
-  env = (@empty type) ->
   typeinf env 0 e (fv, S, C) ->
   solution s C ->
-  (exists (t : t_expr), erase t = e /\ typecheck env t (apply s S)).
+  (exists (t : t_expr), erase t = e /\ typecheck env t (app_substs s S)).
 Proof.
 Admitted.
